ArkLib/OracleReduction/ProtocolSpec/SeqCompose.lean
@@ -383,31 +383,29 @@ instance : ∀ i, OracleInterface ((pSpec₁ ++ₚ pSpec₂).Challenge i) := cha
 
 @[simp]
 lemma challengeOracleInterface_append_domain_inl (j : pSpec₁.ChallengeIdx) :
-    [(pSpec₁ ++ₚ pSpec₂).Challenge (.inl j)]ₒ.domain = Unit := by
-  simp [OracleSpec.domain, ChallengeIdx.inl, ProtocolSpec.append, OracleInterface.toOracleSpec,
-    instOracleInterfaceChallengeAppend, challengeOracleInterface]
+    [(pSpec₁ ++ₚ pSpec₂).Challenge (.inl j)]ₒ.domain = Unit := rfl
 
 @[simp]
 lemma challengeOracleInterface_append_range_inl (j : pSpec₁.ChallengeIdx) :
     [(pSpec₁ ++ₚ pSpec₂).Challenge (.inl j)]ₒ.range () = pSpec₁.Challenge j := by
-  simp [OracleSpec.range, ChallengeIdx.inl, ProtocolSpec.append, OracleInterface.toOracleSpec,
-    instOracleInterfaceChallengeAppend, challengeOracleInterface]
+  simp only [append, ChallengeIdx.inl, Challenge, instOracleInterfaceChallengeAppend,
+    challengeOracleInterface, OracleInterface.toOracleSpec', OracleInterface.toOracleSpec,
+    Fin.vappend_left]
 
 @[simp]
 lemma challengeOracleInterface_append_domain_inr (j : pSpec₂.ChallengeIdx) :
-    [(pSpec₁ ++ₚ pSpec₂).Challenge (.inr j)]ₒ.domain = Unit := by
-  simp [OracleSpec.domain, ChallengeIdx.inr, ProtocolSpec.append, OracleInterface.toOracleSpec,
-    instOracleInterfaceChallengeAppend, challengeOracleInterface]
+    [(pSpec₁ ++ₚ pSpec₂).Challenge (.inr j)]ₒ.domain = Unit := rfl
 
 @[simp]
 lemma challengeOracleInterface_append_range_inr (j : pSpec₂.ChallengeIdx) :
     [(pSpec₁ ++ₚ pSpec₂).Challenge (.inr j)]ₒ.range () = pSpec₂.Challenge j := by
-  simp [OracleSpec.range, ChallengeIdx.inr, ProtocolSpec.append, OracleInterface.toOracleSpec,
-    instOracleInterfaceChallengeAppend, challengeOracleInterface]
+  simp only [append, ChallengeIdx.inr, Challenge, instOracleInterfaceChallengeAppend,
+    challengeOracleInterface, OracleInterface.toOracleSpec', OracleInterface.toOracleSpec,
+    Fin.vappend_right]
 
 variable [∀ i, SampleableType (pSpec₁.Challenge i)] [∀ i, SampleableType (pSpec₂.Challenge i)]
 
--- instance instSubSpecOfProtocolSpecAppendChallenge (j : pSpec₁.ChallengeIdx) (j' : pSpec₂.ChallengeIdx) :
+-- instance instSubSpecOfProtocolSpecAppendChallenge :
 --     SubSpec ([pSpec₁.Challenge j]ₒ + [pSpec₂.Challenge j']ₒ) ([(pSpec₁ ++ₚ pSpec₂).Challenge (by
 --       simp
 --       sorry
@@ -419,10 +417,12 @@ variable [∀ i, SampleableType (pSpec₁.Challenge i)] [∀ i, SampleableType (
 --       simpa using query (spec := [(pSpec₁ ++ₚ pSpec₂).Challenge]ₒ) j.inr ()
 
 -- instance : SubSpec [pSpec₁.Challenge]ₒ ([(pSpec₁ ++ₚ pSpec₂).Challenge]ₒ) where
---   monadLift | query i t => instSubSpecOfProtocolSpecAppendChallenge.monadLift (query (Sum.inl i) t)
+--   monadLift | query i t =>
+--     instSubSpecOfProtocolSpecAppendChallenge.monadLift (query (Sum.inl i) t)
 
 -- instance : SubSpec [pSpec₂.Challenge]ₒ ([(pSpec₁ ++ₚ pSpec₂).Challenge]ₒ) where
---   monadLift | query i t => instSubSpecOfProtocolSpecAppendChallenge.monadLift (query (Sum.inr i) t)
+--   monadLift | query i t =>
+--    instSubSpecOfProtocolSpecAppendChallenge.monadLift (query (Sum.inr i) t)
 
 end Append
 
